[Automata] Add some theorems about execution; fix `invInductive`

LeanSts/TransitionSystem.lean
@@ -31,11 +31,46 @@ class RelationalTransitionSystem (σ : Type) extends
 
 open RelationalTransitionSystem
 
-def invInit [RelationalTransitionSystem σ] :=
-  ∀ (s : σ), init s -> inv s
-
+/-- All states in the invariant are safe. -/
 def invSafe [RelationalTransitionSystem σ] :=
   ∀ (s : σ), inv s -> safe s
 
-def invInductive [RelationalTransitionSystem σ] :=
+/-- The set of initial states are in the invariant. -/
+def invInit [RelationalTransitionSystem σ] :=
+  ∀ (s : σ), init s -> inv s
+
+/-- The invariant is preserved by transition. -/
+def invConsecution [RelationalTransitionSystem σ] :=
   ∀ (s1 s2 : σ), next s1 s2 -> inv s1 -> inv s2
+
+/-- The invariant is inductive. -/
+def invInductive [sys: RelationalTransitionSystem σ] :=
+  @invInit σ sys ∧ @invConsecution σ sys
+
+def validStutteringExecution [RelationalTransitionSystem σ] (e : exec σ) :=
+  init (e 0) ∧ ∀ (i : Nat), (next (e i) (e (i + 1))) ∨ (e i = e (i + 1))
+
+/-- The set of all reachable states of the system. -/
+def reachableStates [RelationalTransitionSystem σ] : σ → Prop :=
+  (λ (s : σ) => ∃ (e : exec σ), validStutteringExecution e ∧ ∃ (step : Nat), s = e step)
+
+theorem init_is_reachable [RelationalTransitionSystem σ] :
+  ∀ (s : σ), init s -> reachableStates s := by
+  intro s hinit; apply Exists.intro (λ _ => s)
+  simp only [validStutteringExecution, or_true, implies_true, and_true, exists_const, hinit]
+
+theorem valid_execution_in_inductive_inv [sys : RelationalTransitionSystem σ] (e : exec σ) :
+  @invInductive σ sys → validStutteringExecution e → ∀ (i : Nat), inv (e i) := by
+  intro ⟨h0, hinv⟩ hvalid i
+  induction i with
+  | zero => { apply h0; apply hvalid.left }
+  | succ i ih => {
+    rcases hvalid.right i with tr | stutter
+    . apply (@hinv _ _ tr); apply ih
+    . rw [stutter] at ih; apply ih
+  }
+
+theorem reachable_in_inductive_inv [sys : RelationalTransitionSystem σ] :
+  @invInductive σ sys → ∀ (s : σ), reachableStates s → inv s := by
+  intro hinv s ⟨exec, ⟨valid, ⟨i, hs⟩⟩⟩; subst s
+  apply valid_execution_in_inductive_inv exec hinv valid i
